Clean up repo, rename some types

src/Env.v
@@ -1,41 +1,67 @@
-Require Export PPS.Map.
-Require Import Lists.List.
-Import ListNotations.
-
 Set Implicit Arguments.
 
-Section Env.
+Section TotalMap.
 
-  Variable ID Val : Type.
-  Variable eqID : ID -> ID -> bool.
-  Notation "i '==' j" := (eqID i j) (at level 80, right associativity).
+  Variable K V : Type.
+  Variable eqK : K -> K -> bool.
+  Notation "i '==' j" := (eqK i j) (at level 80, right associativity).
 
-  Definition EnvironmentP := partialMap ID Val.
-  Definition EnvironmentT := totalMap ID Val.
-  Definition EnvironmentL := list (ID * Val).
+  Definition totalMap := K -> V.
 
-  Fixpoint lookup (Sigma : EnvironmentL) (i : ID) : option Val :=
-    match Sigma with
-    | []          => None
-    | (k,v) :: ps => if (k == i) then Some v
-                    else lookup ps i
+  Definition emptyTMap (v : V) : totalMap := fun _ => v.
+
+  Definition updateTMap (m : totalMap) (k : K) (v : V) :=
+    fun k' => if k == k' then v else m k'.
+
+End TotalMap.
+
+Section PartialMap.
+
+  Variable K V : Type.
+  Variable eqK : K -> K -> bool.
+
+  Definition partialMap := totalMap K (option V).
+
+  Definition emptyPMap : partialMap := emptyTMap None.
+
+  Definition updatePMap (m : partialMap) (k : K) (v : V) :=
+    updateTMap eqK m k (Some v).
+
+End PartialMap.
+
+Section ListMap.
+
+  Variable K V : Type.
+  Variable eqK : K -> K -> bool.
+  Notation "i '==' j" := (eqK i j) (at level 80, right associativity).
+
+  Definition listMap := list (K * V).
+
+  Definition add (kvs : listMap) (k : K) (v : V) : listMap :=
+    cons (k,v) kvs.
+
+  Fixpoint update (kvs : listMap) (k : K) (v : V) : listMap :=
+    match kvs with
+    | nil               => cons (k,v) nil
+    | cons (k',v') kvs' => if (k' == k) then cons (k',v) kvs'
+                          else cons (k',v') (update kvs' k v)
     end.
 
-  Fixpoint update (Sigma : EnvironmentL) (i : ID) (v' : Val) : EnvironmentL :=
-    match Sigma with
-    | []          => [(i,v')]
-    | (k,v) :: ps => if (k == i) then (k,v') :: ps
-                    else (k,v) :: update ps i v'
+  Fixpoint lookup (kvs : listMap) (k : K) : option V :=
+    match kvs with
+    | nil              => None
+    | cons (k',v) kvs' => if (k' == k) then Some v
+                         else lookup kvs' k
     end.
 
-  Definition union (Sigma Delta : EnvironmentL) := app Sigma Delta.
+  Definition union (kvs1 kvs2 : listMap) : listMap := app kvs1 kvs2.
 
-End Env.
+End ListMap.
 
 Section Properties.
 
   Lemma lookup_deterministic :
-    forall (A B : Type) (eqA : A -> A -> bool) (Sigma : EnvironmentL A B) (k : A) (v1 v2 : option B),
+    forall (A B : Type) (eqA : A -> A -> bool) (Sigma : listMap A B) (k : A) (v1 v2 : option B),
       lookup eqA Sigma k = v1 ->
       lookup eqA Sigma k = v2 ->
       v1 = v2.
@@ -46,7 +72,7 @@ Section Properties.
   Qed.
 
   Lemma lookupT_deterministic :
-    forall (A B : Type) (Sigma : EnvironmentT A B) (k : A) (v1 v2 : B),
+    forall (A B : Type) (Sigma : totalMap A B) (k : A) (v1 v2 : B),
       Sigma k = v1 ->
       Sigma k = v2 ->
       v1 = v2.
@@ -57,7 +83,7 @@ Section Properties.
   Qed.
 
   Lemma lookupP_deterministic :
-    forall (A B : Type) (Sigma : EnvironmentP A B) (k : A) (v1 v2 : option B),
+    forall (A B : Type) (Sigma : partialMap A B) (k : A) (v1 v2 : option B),
       Sigma k = v1 ->
       Sigma k = v2 ->
       v1 = v2.
@@ -67,8 +93,55 @@ Section Properties.
     apply H0.
   Qed.
 
-    Lemma update_lookup1 :
-    forall (A B : Type) (eqA : A -> A -> bool) (Sigma : EnvironmentL A B) (k : A) (v : B),
+
+  Lemma update_lookupT1 :
+    forall (A B : Type) (eqA : A -> A -> bool) (Sigma : totalMap A B) (k : A) (v : B),
+      (forall x : A, eqA x x = true) ->
+      (updateTMap eqA Sigma k v) k = v.
+  Proof.
+    intros.
+    unfold updateTMap.
+    rewrite (H k).
+    reflexivity.
+  Qed.
+
+  Lemma update_lookupT2 :
+    forall (A B : Type) (eqA : A -> A -> bool) (Sigma : totalMap A B) (k1 k2 : A) (v1 v2 : B),
+      eqA k2 k1 = false ->
+      (updateTMap eqA Sigma k2 v2) k1 = Sigma k1.
+  Proof.
+    intros.
+    unfold updateTMap.
+    rewrite H.
+    reflexivity.
+  Qed.
+
+  Lemma add_lookupL1 :
+    forall (A B : Type) (eqA : A -> A -> bool) (Sigma : listMap A B) (k : A) (v : B),
+      (forall x : A, eqA x x = true) ->
+      lookup eqA (add Sigma k v) k = Some v.
+  Proof.
+    intros.
+    unfold add.
+    simpl lookup.
+    rewrite (H k).
+    reflexivity.
+  Qed.
+
+  Lemma add_lookupL2 :
+    forall (A B : Type) (eqA : A -> A -> bool) (Sigma : listMap A B) (k1 k2 : A) (v  : B),
+      eqA k2 k1 = false ->
+      lookup eqA (add Sigma k2 v) k1 = lookup eqA Sigma k1.
+  Proof.
+    intros.
+    unfold add.
+    simpl lookup.
+    rewrite H.
+    reflexivity.
+  Qed.    
+
+  Lemma update_lookup1 :
+    forall (A B : Type) (eqA : A -> A -> bool) (Sigma : listMap A B) (k : A) (v : B),
       (forall x : A, eqA x x = true) ->
       lookup eqA (update eqA Sigma k v) k = Some v.
   Proof.
@@ -76,48 +149,44 @@ Section Properties.
     induction Sigma; simpl.
     - rewrite (H k).
       reflexivity.
-    - destruct a.
-      remember (eqA a k) as akBool.
-      destruct akBool.
-      + simpl.
-        rewrite <- HeqakBool.
+    - destruct a as [k' v'].
+      destruct (eqA k' k) eqn:HeqKK.
+      + simpl lookup.
+        rewrite HeqKK.
         reflexivity.
-      + simpl.
-        rewrite <- HeqakBool.
+      + simpl lookup.
+        rewrite HeqKK.
         apply IHSigma.
   Qed.
 
   Lemma update_lookup2 :
-    forall (A B : Type) (eqA : A -> A -> bool) (Sigma : EnvironmentL A B) (k1 k2 : A) (v1 v2 : B),
+    forall (A B : Type) (eqA : A -> A -> bool) (Sigma : listMap A B) (k1 k2 : A) (v : B),
       (forall x y z : A, eqA x y = eqA x z -> true = eqA y z) ->
       eqA k2 k1 = false ->
-      lookup eqA (update eqA Sigma k2 v2) k1 = lookup eqA Sigma k1.
+      lookup eqA (update eqA Sigma k2 v) k1 = lookup eqA Sigma k1.
   Proof.
     intros.
     induction Sigma; simpl.
     - rewrite H0.
       reflexivity.
-    - destruct a as [ k v ].
-      remember (eqA k k2) as kk2Bool.
-      destruct kk2Bool.
-      + simpl.
-        remember (eqA k k1) as kk1Bool.
-        destruct kk1Bool.
-        * rewrite Heqkk2Bool in Heqkk1Bool.
-          specialize (H k k2 k1 Heqkk1Bool).
+    - destruct a as [k' v'].
+      destruct (eqA k' k2) eqn:HeqKK2.
+      + simpl lookup.
+        destruct (eqA k' k1) eqn:HeqKK1.
+        * rewrite <- HeqKK1 in HeqKK2.
+          specialize (H k' k2 k1 HeqKK2).
           congruence.
         * reflexivity.
-      + simpl.
-        remember (eqA k k1) as kk1Bool.
-        destruct kk1Bool.
+      + simpl lookup.
+        destruct (eqA k' k1) eqn:HeqKK1.
         * reflexivity.
         * apply IHSigma.
   Qed.
 
   Lemma union_lookup :
-    forall (A B : Type) (eqA : A -> A -> bool) (Sigma Delta : EnvironmentL A B) (k : A),
-      lookup A B eqA Delta k = None ->
-      lookup A B eqA (union A B Delta Sigma ) k = lookup A B eqA Sigma k.
+    forall (A B : Type) (eqA : A -> A -> bool) (Sigma Delta : listMap A B) (k : A),
+      lookup eqA Delta k = None ->
+      lookup eqA (union Delta Sigma ) k = lookup eqA Sigma k.
   Proof.
     intros.
     induction Delta; simpl.
